polymorphic hreduce!

test/Test_Kuiper_HReduceF32Plus.cu
@@ -19,7 +19,7 @@ int main()
 
 	MUST(cudaMemcpy(ga, a, siz * sizeof(float), cudaMemcpyHostToDevice));
 
-	KPR_KCALL(Kuiper_HReduceF32Plus_k_reduce, 1, siz, siz, ga);
+	Kuiper_HReduceF32Plus_reduce(siz, ga);
 
 	MUST(cudaMemcpy(a, ga, siz * sizeof(float), cudaMemcpyDeviceToHost));
 	MUST(cudaFree(ga));
