src/lib/kernels/Kuiper.HReduceU32Plus.fsti
@@ -3,108 +3,11 @@ module Kuiper.HReduceU32Plus
 #lang-pulse
 
 open Kuiper
-open Kuiper.Barrier.RPM
-open Kuiper.Math
-open Kuiper.Seq.Common
-open Kuiper.IsReduction
+open Kuiper.HReduce
 
-module SZ = FStar.SizeT
-module F = FStar.UInt32
+let size = 1024sz (* crutch *)
 
-let size : sz = 1024sz
-
-(* no polymorphism, but at least keep the definitions here *)
-let ety = F.t
-inline_for_extraction noextract let op  : ety -> ety -> ety = F.add_mod
-inline_for_extraction noextract let neu : ety = F.zero
-
-(* Ownership of array r between i and j. The first value of that slice
-is the reduction of all the values in the (original) slice v. *)
-unfold
-let gpu_pts_to_slice_sum_inner
-  (#sz:nat)
-  (r : gpu_array ety sz)
-  (i j :nat)
-  (v : seq ety)
-  (s : seq ety)
-: slprop
-= gpu_pts_to_slice r i j s
-  ** pure (i < j /\ j <= sz /\
-           len v = sz /\
-           len s = j - i /\
-           squash (is_reduction neu op (Seq.slice v i j) (s @! 0))) // SQUASH VERY IMPORTANT!!
-
-(* Not easy to mark this unfold as it has a lambda (in the exists) *)
-let gpu_pts_to_slice_sum
-  (#sz:nat)
-  ([@@@mkey] r: gpu_array ety sz)
-  ([@@@mkey] i : nat)
-  (j:nat)
-  (v: seq ety)
-: slprop
-= if_ (i < j && j <= sz) (exists* s. gpu_pts_to_slice_sum_inner #sz r i j v s)
-
-// Barrier
-
-val barrier_matrix (nth: nat) (r : gpu_array ety nth) (v: seq ety) (it from to: nat)
-  : slprop
-
-unfold
-let kpre (nth: nat) (a : gpu_array ety nth) (s : erased (seq ety))
-  (#_: squash (len s == nth)) (tid:nat{tid < nth})
-  : slprop =
-    gpu_pts_to_slice a tid (tid+1) seq![Seq.index s tid]
-
-unfold
-let kpost (nth: nat) (a : gpu_array ety nth) (s : erased (seq ety))
-  (#_: squash (len s == nth)) (tid:nat{tid < nth})
-  : slprop =
-    if_ (tid = 0) (gpu_pts_to_slice_sum a 0 nth s)
-
-[@@ CPrologue "__device__"]
-inline_for_extraction
-fn d_reduce
-  (nth : sz { 0 < SZ.v nth /\ SZ.v nth <= 1024 })
-  (a : gpu_array ety nth)
-  (#s :  erased (seq ety))
-  (#_: squash (len s == nth))
-  (etid : tid_t { (gdim_x etid <: nat) == 1ul /\ (bdim_x etid <: nat) == SZ.sizet_to_uint32 nth })
-  preserves
-    gpu ** thread_id etid
-  requires
-    mbarrier_tok nth (barrier_matrix nth a s) 0 (tidx_x etid) **
-    kpre nth a s (thread_index etid)
-  ensures
-    exists* it.
-      mbarrier_tok nth (barrier_matrix nth a s) it (tidx_x etid) **
-      kpost nth a s (thread_index etid)
-
-(* NB: cannot use 'preserves' as we depend on the shape of pre/post *)
-[@@ CPrologue "__global__"]
-inline_for_extraction
-fn k_reduce
-  (nth : sz { 0 < SZ.v nth /\ SZ.v nth <= 1024 })
-  (a : gpu_array ety nth)
-  (#s :  erased (seq ety))
-  (#_: squash (len s == nth))
-  (etid : tid_t { (gdim_x etid <: nat) == 1ul /\ (bdim_x etid <: nat) == SZ.sizet_to_uint32 nth })
-  requires
-    gpu **
-    thread_id etid **
-    mbarrier_tok nth (barrier_matrix nth a s) 0 (tidx_x etid) **
-    kpre nth a s (thread_index etid)
-  ensures
-    gpu **
-    thread_id etid **
-    (exists* it. mbarrier_tok nth (barrier_matrix nth a s) it (tidx_x etid)) **
-    kpost nth a s (thread_index etid)
-
-fn reduce
-  (lena : szp { lena < max_threads })
-  (a : gpu_array ety lena)
-  requires
-    cpu **
-    gpu_pts_to_array a 'va
-  ensures
-    cpu **
-    (exists* va'. gpu_pts_to_array a va') (* underspec *)
+inline_for_extraction noextract
+val d_reduce : k_reduce_ty u32
+val k_reduce : k_reduce_ty u32
+val reduce : reduce_ty u32
