src/lib/kernels/Kuiper.HReduce.fst
@@ -1,0 +1,350 @@
+module Kuiper.HReduce
+
+#lang-pulse
+
+open Kuiper
+open Kuiper.Barrier.RPM
+open Kuiper.Math
+open Kuiper.Seq.Common
+
+module SZ = FStar.SizeT
+module U32 = FStar.UInt32
+
+[@@ CPrologue "__device__"]
+noextract inline_for_extraction
+let spow2 (s : sz{s < 32}) : r:sz{SZ.v r == pow2 (SZ.v s)} =
+  (* Computing 2^s by 1<<s *)
+  SZ.uint32_to_sizet (U32.shift_left 1ul (sizet_to_u32 s))
+
+[@@ CPrologue "__device__"]
+noextract inline_for_extraction
+let sdiv_pow2 (i:sz{i < 32}) (tid: sz) : bool =
+  // SZ.rem tid (spow2 i) = 0sz
+  sizet_and tid SZ.(spow2 i -^ 1sz) = 0sz
+
+let sdiv_pow2_ok (i:sz{i < 32}) (tid:sz) :
+  Lemma (sdiv_pow2 i tid <==> div_pow2 (SZ.v i) (SZ.v tid))
+        [SMTPat (sdiv_pow2 i tid)]
+= sizet_and_div_pow2 tid (spow2 i) i;
+  calc (==) {
+    SZ.v (SZ.rem tid (spow2 i));
+    == {}
+    SZ.v tid - ((SZ.v tid / SZ.v (spow2 i)) * SZ.v (spow2 i));
+    == { FStar.Math.Lemmas.euclidean_division_definition (SZ.v tid) (SZ.v (spow2 i)) }
+    SZ.v tid % SZ.v (spow2 i);
+    == {}
+    SZ.v tid % pow2 (SZ.v i);
+}
+
+[@@ CPrologue "__device__"]
+noextract inline_for_extraction
+let smin (a b : sz): sz =
+  let open FStar.SizeT in
+  if a <^ b then a else b
+
+// Barrier
+
+let barrier_matrix
+  (#et:Type0) {| simple_scalar et |}
+  (nth : nat) (r : gpu_array et nth)
+  (v : seq et)
+  (it from to : nat)
+: slprop
+=
+  if_ (from = to + pow2 it)
+      (if_ (not (div_pow2 (it + 1) from) && (div_pow2 it from))
+           (gpu_pts_to_slice_sum r from (min (from + pow2 it) nth) v))
+
+ghost
+fn fold_barrier_matrix_true
+  (#et:Type0) {| simple_scalar et |}
+  (nth : nat)
+  (r: gpu_array et nth)
+  (v: seq et { len v == nth })
+  (it: nat)
+  (tid: nat { tid <= nth /\ tid >= pow2 it })
+  (to: nat)
+  requires if_ (to = tid - pow2 it)
+             (if_ (not (div_pow2 (it + 1) tid) && div_pow2 it tid)
+               (gpu_pts_to_slice_sum r tid (min (tid + pow2 it) nth) v))
+  ensures  barrier_matrix nth r v it tid to
+{
+  fold (barrier_matrix nth r v it tid to);
+}
+
+ghost
+fn fold_barrier_matrix_false
+  (#et:Type0) {| simple_scalar et |}
+  (nth : nat)
+  (r: gpu_array et nth)
+  (v: seq et { len v == nth })
+  (it: nat)
+  (tid: nat { tid <= nth /\ tid < pow2 it })
+  (to: nat { to <= nth })
+  requires emp
+  ensures  barrier_matrix nth r v it tid to
+{
+  assert (pure (tid < to + pow2 it /\ not (tid = to + pow2 it)));
+  if_intro_false (if_ (not (div_pow2 (it + 1) tid) && (div_pow2 it tid)) (gpu_pts_to_slice_sum r tid (min (tid + pow2 it) nth) v));
+  // (tid = to + pow2 it)
+  fold (barrier_matrix nth r v it tid to);
+}
+
+// #push-options "--print_implicits --print_bound_var_types"
+
+ghost
+fn mk_barrier_pre
+  (#et:Type0) {| simple_scalar et |}
+  (nth : sz { 0 < SZ.v nth /\ SZ.v nth <= 1024 })
+  (r : gpu_array et nth)
+  (vv: erased (seq et))
+  (#_: squash (len vv == nth))
+  (tid : sz{SZ.v tid < nth})
+  (it: sz{it < 31})
+  requires if_ (not (div_pow2 (it + 1) tid) && div_pow2 it tid)
+      (gpu_pts_to_slice_sum r tid (min (tid + pow2 it) nth) vv)
+  ensures bigstar 0 nth (barrier_matrix nth r vv it tid)
+{
+  open FStar.SizeT;
+  if (tid >=^ spow2 it) {
+    bigstar_if_intro 0 nth (tid - pow2 it) (fun _ -> if_ (not (div_pow2 (it + 1) tid) && (div_pow2 it tid)) (gpu_pts_to_slice_sum r tid (min (tid + pow2 it) nth) vv));
+    bigstar_map #_ #_ #0 #nth #(fun (i:nat { 0 <= i /\ i < nth }) -> _ i) (fold_barrier_matrix_true nth r vv it tid);
+  } else {
+    FStar.Math.Lemmas.modulo_lemma tid (spow2 it);
+    FStar.Math.Lemmas.modulo_lemma 0 (spow2 (it +^ 1sz));
+    // assert (pure ((tid <: nat) <> 0 ==> not (div_pow2 it tid)));
+    // assert (pure ((tid <: nat) = 0 ==> (div_pow2 (it + 1) tid)));
+    if_rewrite_bool (op_Negation (div_pow2 (SZ.v it + 1) (SZ.v tid)) && div_pow2 (SZ.v it) (SZ.v tid)) false _;
+    if_elim_false _;
+
+    bigstar_emp_intro 0 nth;
+    bigstar_map #_ #_ #0 #nth #(fun (i:nat { 0 <= i /\ i < nth }) -> emp) (fold_barrier_matrix_false nth r vv it tid);
+  }
+}
+
+// KrmlPrivate is essentially a "noextract". F* usually adds it
+// automatically to any definition that does not appear in the fsti,
+// but we have disable that since it interoperates poorly with pulse
+// (due to splicing).
+[@@ CPrologue "__device__"; "KrmlPrivate"]
+inline_for_extraction
+fn iteration
+  (#et:Type0) {| simple_scalar et |}
+  (nth : sz { 0 < SZ.v nth /\ SZ.v nth <= 1024 })
+  (r : gpu_array et nth)
+  (vv: erased (seq et))
+  (#_: squash (len vv == nth))
+  (tid : sz{SZ.v tid < nth})
+  (it: sz{it < 31})
+  requires gpu
+    ** mbarrier_tok nth (barrier_matrix nth r vv) it tid
+    ** if_ (div_pow2 it tid) (gpu_pts_to_slice_sum r tid (min (tid + pow2 it) nth) vv)
+  ensures gpu
+    ** mbarrier_tok nth (barrier_matrix nth r vv) (it+1) tid
+    ** if_ (div_pow2 (it+1) tid) (gpu_pts_to_slice_sum r tid (min (tid + pow2 (it + 1)) nth) vv)
+{
+  assert (pure (len vv = nth));
+
+  case_split (div_pow2 (it + 1) tid) (if_ (div_pow2 it tid) (gpu_pts_to_slice_sum r tid (min (tid + pow2 it) nth) vv));
+  if_flatten #(div_pow2 (it + 1) tid);
+  if_flatten #(not (div_pow2 (it + 1) tid));
+
+  div_pow2_lemma it (it + 1) tid;
+  rewrite (if_ (div_pow2 (it + 1) tid && div_pow2 it tid)
+            (gpu_pts_to_slice_sum r tid (min (tid + pow2 it) nth) vv))
+      as (if_ (div_pow2 (it + 1) tid)
+            (gpu_pts_to_slice_sum r tid (min (tid + pow2 it) nth) vv));
+
+  mk_barrier_pre nth r vv tid it;
+  mbarrier_wait #(SZ.v nth) #(barrier_matrix nth r vv) #(SZ.v it) #(SZ.v tid);
+
+  ghost fn aux (from : nat)
+    requires barrier_matrix nth r vv it from tid
+    ensures  if_ (from = tid + pow2 it) (
+               if_ (not (div_pow2 (it + 1) from) && (div_pow2 it from)) (
+                 gpu_pts_to_slice_sum r from (min (from + pow2 it) nth) vv
+             ))
+  {
+    (* FIXME: bad crash if we just say 'unfold barrier_matrix' *)
+    unfold barrier_matrix nth r vv it from tid;
+  };
+  bigstar_map #_ #_ #0 #nth (fun (from: nat { 0 <= from /\ from < nth }) -> aux from );
+
+  // combine (div_pow2 (it + 1) tid) (gpu_pts_to_slice_sum r tid (min (tid + pow2 it) nth) vv) _;
+
+  let nextid = FStar.SizeT.(tid +^ spow2 it);
+
+  (* We do not use end_ in extracted code, so we can use a nat and erase it
+  so there are no traces in the extracted C. *)
+  let end_   : erased nat = hide (min (tid + 2 * pow2 it) nth);
+
+  if (FStar.SizeT.(nextid <^ nth)) {
+    bigstar_if_elim #_ #0
+      #nth (tid + pow2 it)
+      (fun (from: nat) -> if_ (not (div_pow2 (it + 1) from) && (div_pow2 it from)) (gpu_pts_to_slice_sum r from (min (from + pow2 it) nth) vv));
+
+    let b = sdiv_pow2 (FStar.SizeT.(it +^ 1sz)) tid;
+
+    rewrite each (div_pow2 (SZ.v it + 1) (SZ.v tid)) as b;
+
+    div_pow2_lemma_2 it tid;
+    combine
+      b
+      (gpu_pts_to_slice_sum r nextid (min (tid + pow2 it + pow2 it) nth) vv)
+      _;
+
+    if b {
+      assert (pure (div_pow2 (SZ.v it + 1) (SZ.v tid)));
+      if_elim_true _;
+
+      (**)unfold (gpu_pts_to_slice_sum #et r tid nextid vv);
+      (**)if_elim_true (exists* s. gpu_pts_to_slice_sum_inner r tid nextid vv s);
+      let s1 = gpu_array_read #et #_ #tid #nextid r tid;
+      (**)assert (pure (squash (is_reduction #et Scalars.zero Scalars.add (Seq.slice vv tid nextid) s1)));
+
+      (**)unfold (gpu_pts_to_slice_sum r nextid end_ vv);
+      (**)if_elim_true (exists* s. gpu_pts_to_slice_sum_inner r nextid end_ vv s);
+      let s2 = gpu_array_read #_ #_ #nextid #end_ r nextid;
+      (**)assert (pure (squash (is_reduction zero add (Seq.slice vv nextid end_) s2)));
+
+      let s = add s1 s2;
+      (**)lem_append_slice vv tid nextid end_;
+      (**)assert (pure (squash (is_reduction zero add (Seq.slice vv tid end_) s)));
+
+      gpu_array_write #et #(SZ.v nth) #(SZ.v tid) #(SZ.v nextid) r tid s;
+
+      (**)gpu_slice_concat #et #(SZ.v nth) r tid nextid end_;
+      (**)with seq. assert (gpu_pts_to_slice r tid end_ seq);
+      (**)if_intro_true (exists* s. gpu_pts_to_slice_sum_inner r tid end_ vv s);
+      (**)fold (gpu_pts_to_slice_sum r tid end_ vv);
+      (**)if_intro_true (gpu_pts_to_slice_sum r tid end_ vv);
+      (**)rewrite
+      (**)  if_ true (gpu_pts_to_slice_sum r (SZ.v tid) (reveal end_) (reveal vv))
+      (**)as
+      (**)  if_ (div_pow2 (SZ.v it + 1) (SZ.v tid))
+      (**)    (gpu_pts_to_slice_sum r
+      (**)        (SZ.v tid)
+      (**)        (min (SZ.v tid + pow2 (SZ.v it + 1)) (SZ.v nth))
+      (**)        (reveal vv));
+      ();
+    } else {
+      if_elim_false _;
+      if_intro_false (gpu_pts_to_slice_sum r tid end_ vv);
+    }
+  } else {
+    bigstar_map #_ #_ #0 #nth #(fun (from:nat { 0 <= from /\ from < nth }) -> _ from)
+      (fun (from: nat{0 <= from /\ from < nth}) ->
+        if_rewrite_bool (from = tid + pow2 it) false _);
+    bigstar_map #_ #_ #0 #nth #(fun (from:nat { 0 <= from /\ from < nth }) -> _ from)
+      (fun (from: nat{0 <= from /\ from < nth}) ->
+        if_elim_false (if_ (not (div_pow2 (it + 1) from) && (div_pow2 it from)) (gpu_pts_to_slice_sum r from (min (from + pow2 it) nth) vv)));
+    bigstar_emp_elim #_;
+  }
+}
+
+inline_for_extraction noextract
+fn d_reduce
+  (#et:Type0) {| simple_scalar et |}
+  (nth : szp { nth <= 1024 })
+  (a : gpu_array et nth)
+  (#s :  erased (seq et))
+  (#_ : squash (Seq.length s == nth))
+  (etid : tid_t { (gdim_x etid <: nat) == 1 /\ (bdim_x etid <: nat) == SZ.v nth })
+  requires
+    gpu ** thread_id etid **
+    mbarrier_tok nth (barrier_matrix nth a s) 0 (tidx_x etid) **
+    kpre nth a s (thread_index etid)
+  ensures
+    gpu ** thread_id etid **
+    (exists* it.  mbarrier_tok nth (barrier_matrix nth a s) it (tidx_x etid)) **
+    kpost nth a s (thread_index etid)
+{
+  let tid = thread_idx_x ();
+  rewrite each thread_index etid as tid;
+
+  (* Reduction *)
+  let mut n = 0sz;
+
+  (**)with ss. assert (gpu_pts_to_slice a tid (tid+1) ss);
+  assert (pure (Seq.slice s tid (tid+1) `Seq.equal` seq![ss @! 0])); // sucks
+  (**)if_intro_true (exists* ss. gpu_pts_to_slice_sum_inner a tid (tid + pow2 0) s ss);
+  (**)fold (gpu_pts_to_slice_sum a tid (tid + pow2 0) s);
+  (**)if_intro_true (gpu_pts_to_slice_sum a tid (tid + pow2 0) s);
+
+  open FStar.SizeT;
+  while (let it = !n; (spow2 it <^ nth))
+    invariant c.
+      exists* (it:sz).
+        gpu **
+        pts_to n it **
+        mbarrier_tok nth (barrier_matrix nth a s) it tid **
+        if_ (div_pow2 (SZ.v it) (SZ.v tid)) (gpu_pts_to_slice_sum a tid (min (tid + pow2 it) nth) s) **
+        pure (c == (pow2 it < nth) /\ SZ.v it < 32)
+  {
+    let it = !n;
+    iteration nth a s tid it;
+    n := it +^ 1sz;
+  };
+}
+
+inline_for_extraction noextract
+fn k_reduce
+  (#et:Type0) {| simple_scalar et |}
+  (nth : szp { nth <= 1024 })
+  (a : gpu_array et nth)
+  (#s :  erased (seq et))
+  (#_: squash (len s == nth))
+  (etid : tid_t { (gdim_x etid <: nat) == 1ul /\ (bdim_x etid <: nat) == SZ.sizet_to_uint32 nth })
+  requires
+    gpu **
+    thread_id etid **
+    mbarrier_tok nth (barrier_matrix nth a s) 0 (tidx_x etid) **
+    kpre nth a s (thread_index etid)
+  ensures
+    gpu **
+    thread_id etid **
+    (exists* it. mbarrier_tok nth (barrier_matrix nth a s) it (tidx_x etid)) **
+    kpost nth a s (thread_index etid)
+{
+  d_reduce nth a #s etid;
+}
+
+inline_for_extraction noextract
+fn reduce
+  (#et:Type0) {| simple_scalar et |}
+  (kk : k_reduce_ty et #_)
+  (lena : szp { lena < max_threads })
+  (a : gpu_array et lena)
+  requires
+    cpu **
+    gpu_pts_to_array a 'va
+  ensures
+    cpu **
+    (exists* va'. gpu_pts_to_array a va') (* underspec *)
+{
+  gpu_pts_to_ref a; (* recall length, automate *)
+
+  Array.gpu_array_slice_1 a;
+
+  rewrite each SZ.v lena as (1 * SZ.v lena);
+
+  launch_kernel_n_m_barrier 1sz lena
+    #(kpre  lena a 'va)
+    #(kpost lena a 'va)
+    (fun etid -> kk lena a etid);
+
+  bigstar_extract 0 (1 `op_Multiply` lena) (kpost lena a 'va) 0;
+  if_elim_true _;
+
+  unfold (gpu_pts_to_slice_sum a 0 lena 'va);
+  // if_elim_true _;
+  (* ^ Bad unification from matching, instead of trying to prove that the condition
+     of if_ p f is true (to match it with if_ true ?u) it picks ?u = if_ p f. *)
+  with pp ff. assert (if_ pp ff);
+  rewrite each pp as true;
+  if_elim_true _;
+  bigstar_emp_elim #_ #0 #0;
+  bigstar_emp_elim' #_ #1 #(1 `op_Multiply` lena) _;
+
+  ()
+}
