src/lib/kernels/Kuiper.HReduce.fsti
@@ -1,0 +1,112 @@
+module Kuiper.HReduce
+
+#lang-pulse
+
+open Kuiper
+open Kuiper.Barrier.RPM
+open Kuiper.Math
+open Kuiper.Seq.Common
+open Kuiper.IsReduction
+
+module SZ = FStar.SizeT
+
+let size : sz = 1024sz
+
+(* Ownership of array r between i and j. The first value of that slice
+is the reduction of all the values in the (original) slice v. *)
+unfold
+let gpu_pts_to_slice_sum_inner
+  (#et:Type0) {| simple_scalar et |}
+  (#sz:nat)
+  (r : gpu_array et sz)
+  (i j :nat)
+  (v : seq et)
+  (s : seq et)
+: slprop
+= gpu_pts_to_slice r i j s
+  ** pure (i < j /\ j <= sz /\
+           len v = sz /\
+           len s = j - i /\
+           squash (is_reduction zero add (Seq.slice v i j) (s @! 0))) // SQUASH VERY IMPORTANT!!
+
+(* Not easy to mark this unfold as it has a lambda (in the exists) *)
+let gpu_pts_to_slice_sum
+  (#et:Type0) {| simple_scalar et |}
+  (#sz:nat)
+  ([@@@mkey] r: gpu_array et sz)
+  ([@@@mkey] i : nat)
+  (j:nat)
+  (v: seq et)
+: slprop
+= if_ (i < j && j <= sz) (exists* s. gpu_pts_to_slice_sum_inner r i j v s)
+
+// Barrier
+
+val barrier_matrix
+  (#et:Type0) {| simple_scalar et |}
+  (nth: nat) (r : gpu_array et nth)
+  (v: seq et)
+  (it from to: nat)
+  : slprop
+
+unfold
+let kpre
+  (#et:Type0) {| simple_scalar et |}
+  (nth: nat) (a : gpu_array et nth) (s : erased (seq et))
+  (#_: squash (len s == nth)) (tid:nat{tid < nth})
+  : slprop =
+    gpu_pts_to_slice a tid (tid+1) seq![Seq.index s tid]
+
+unfold
+let kpost 
+  (#et:Type0) {| simple_scalar et |}
+  (nth: nat) (a : gpu_array et nth) (s : erased (seq et))
+  (#_: squash (len s == nth)) (tid:nat{tid < nth})
+  : slprop =
+    if_ (tid = 0) (gpu_pts_to_slice_sum a 0 nth s)
+
+unfold
+type k_reduce_ty (et:Type0) {| simple_scalar et |} =
+  (nth : szp { nth <= 1024 }) ->
+  (a : gpu_array et nth) ->
+  (#s :  erased (seq et)) ->
+  (#_: squash (Seq.length s == SZ.v nth)) ->
+  (etid : tid_t { (gdim_x etid <: nat) == 1 /\ (bdim_x etid <: nat) == SZ.v nth }) ->
+  stt unit
+  (requires
+    gpu **
+    thread_id etid **
+    mbarrier_tok nth (barrier_matrix nth a s) 0 (tidx_x etid) **
+    kpre nth a s (thread_index etid))
+  (ensures fun _ ->
+    gpu **
+    thread_id etid **
+    (exists* it. mbarrier_tok nth (barrier_matrix nth a s) it (tidx_x etid)) **
+    kpost nth a s (thread_index etid))
+
+inline_for_extraction noextract
+val d_reduce (#et:Type0) {| simple_scalar et |} : k_reduce_ty et
+inline_for_extraction noextract
+val k_reduce (#et:Type0) {| simple_scalar et |} : k_reduce_ty et
+
+(* FIXME!!!!!!! Type must unfold or we get weird extracted C.
+e.g. this
+  void ( *Kuiper_HReduceU64Plus2_reduce_u64(size_t lena, uint64_t *a))(size_t x0, uint64_t *x1)
+instead of 
+  void Kuiper_HReduceU64Plus2_reduce_u64(size_t lena, uint64_t *a)
+*)
+unfold
+type reduce_ty (et:Type0) {| simple_scalar et |} =
+  (lena : szp { lena < max_threads }) ->
+  (a : gpu_array et lena) ->
+  (#va : erased (seq et)) ->
+  stt unit 
+  (requires 
+    cpu **
+    gpu_pts_to_array a va)
+  (ensures fun _ ->
+    cpu **
+    (exists* va'. gpu_pts_to_array a va'))
+
+inline_for_extraction noextract
+val reduce (#et:Type0) {| simple_scalar et |} (kk : k_reduce_ty et #_) : reduce_ty et
